src/Formalism/HSE.v
@@ -1,57 +1,64 @@
+Require Import Program.
 Require Import Coq.Sets.Ensembles.
 
 Require Import SpecCert.Formalism.Security.
 Require Import SpecCert.Formalism.Isolation.
 Require Import SpecCert.Formalism.ComputingSystem.
 
+Program Definition software_only_prop
+        {H E: Type}
+       `{Event E}
+        (prop: H -> { e: E | software e } -> Prop)
+        (h: H)
+        (e: E)
+  : Prop :=
+  if software_dec e
+  then prop h e
+  else True.
+
 Record HSEMechanism
-       {H Es Eh: Type}
-       (S:       Type)
-       (C:       ComputingSystem H Es Eh) :=
+       {H E: Type}
+      `{Event E}
+       (S:   Type)
+       (C:   ComputingSystem H E) :=
   { state_inv: H -> Prop
-  ; behavior:  H -> Es -> Prop
+  ; behavior:  H -> { e: E | software e } -> Prop
   ; TCB:       Ensemble S
   ; context:   HardwareSoftwareMapping H S
-  ; behavior_preserves_state_inv:
-      forall h h': H, forall ev: Event Es Eh,
+  ; preserves_state_inv:
+      forall h h': H, forall ev: E,
           state_inv h
-          -> match ev with
-            | software es => behavior h es
-            | _ => True
-            end
           -> precondition C h ev
+          -> software_only_prop behavior h ev
           -> postcondition C h ev h'
           -> state_inv h'
   ; behavior_only_restricts_TCB:
-      forall x: S, forall h: H, forall es: Es,
+      forall x: S, forall h: H, forall es: { e: E | software e },
             ~In S TCB x
             -> context h = x
             -> behavior h es }.
 
-Arguments state_inv [H Es Eh S C] (_ _).
-Arguments behavior [H Es Eh S C] (_ _ _).
-Arguments TCB [H Es Eh S C] (_ _).
-Arguments context [H Es Eh S C] (_ _).
-Arguments behavior_preserves_state_inv [H Es Eh S C] (_ _ _ _ _ _ _ _).
-Arguments behavior_only_restricts_TCB [H Es Eh S C] (_ _ _ _ _ _).
+Arguments state_inv [H E _ S C] (_ _).
+Arguments behavior [H E _ S C] (_ _ _).
+Arguments TCB [H E _ S C] (_ _).
+Arguments context [H E _ S C] (_ _).
+Arguments preserves_state_inv [H E _ S C] (_ _ _ _ _ _ _ _).
+Arguments behavior_only_restricts_TCB [H E _ S C] (_ _ _ _ _ _).
 
-Definition behavior_enforced_step
-           {H Es Eh: Type}
-           {S:       Type}
-           {C:       ComputingSystem H Es Eh}
+Program Definition behavior_enforced_step
+           {H E S:   Type}
+          `{Event E}
+           {C:       ComputingSystem H E}
            (D:       HSEMechanism S C)
            (init:    H)
-           (ev:      Event Es Eh)
+           (ev:      E)
   : Prop :=
-  match ev with
-  | software es => behavior D init es
-  | _           => True
-  end.
+  software_only_prop (behavior D) init ev.
 
 Definition compliant_run
-           {H Es Eh:   Type}
-           {S:         Type}
-           {C:         ComputingSystem H Es Eh}
+           {H E S:     Type}
+          `{Event E}
+           {C:         ComputingSystem H E}
            {init last: H}
            (D:         HSEMechanism S C)
            (r:         Run C init last)
@@ -59,9 +66,9 @@ Definition compliant_run
   state_inv D init /\ always_true (behavior_enforced_step D) r.
 
 Definition sound_mechanism
-           {H Es Eh:   Type}
-           {S:         Type}
-           {C:         ComputingSystem H Es Eh}
+           {H E S  :   Type}
+          `{Event E}
+           {C:         ComputingSystem H E}
            {init last: H}
            (D:         HSEMechanism S C)
            (Psec:      SecurityProperty C init last)
@@ -69,13 +76,14 @@ Definition sound_mechanism
   forall r: Run C init last, compliant_run D r -> Psec r.
 
 Lemma always_true_unwrap
-      {St Es Eh S: Type}
-      {C:          ComputingSystem St Es Eh}
-      {i l p:      St}
-      (prop:       St -> Event Es Eh -> Prop)
-      (ev:         Event Es Eh)
-      (Hst:        state_transformation C p ev l)
-      (r:          Run C i p):
+      {H E:   Type}
+     `{Event E}
+      {C:     ComputingSystem H E}
+      {i l p: H}
+      (prop:  H -> E -> Prop)
+      (ev:    E)
+      (Hst:   p -[C|ev]-> l)
+      (r:     Run C i p):
   always_true prop (sequence r ev Hst)
   -> always_true prop r.
 Proof.
@@ -85,13 +93,14 @@ Proof.
 Qed.
 
 Lemma compliant_run_unwrap
-      {St Es Eh S: Type}
-      {C:          ComputingSystem St Es Eh}
-      {i l p:      St}
-      (D:          HSEMechanism S C)
-      (ev:         Event Es Eh)
-      (Hst:        state_transformation C p ev l)
-      (r:          Run C i p):
+      {H E S: Type}
+     `{Event E}
+      {C:     ComputingSystem H E}
+      {i l p: H}
+      (D:     HSEMechanism S C)
+      (ev:    E)
+      (Hst:   p -[C|ev]-> l)
+      (r:     Run C i p):
   compliant_run D (sequence r ev Hst)
   -> compliant_run D r.
 Proof.
@@ -99,28 +108,29 @@ Proof.
   inversion Hal as [Hprop Hal'].
   unfold compliant_run.
   split; [exact Hprop|].
-  apply (always_true_unwrap (S:=S) (behavior_enforced_step D) ev Hst ) in Hal'.
+  apply (always_true_unwrap (behavior_enforced_step D) ev Hst) in Hal'.
   exact Hal'.
 Qed.
 
 Lemma compliant_run_preserves_inv
-      {St Es Eh S: Type}
-      {C:          ComputingSystem St Es Eh}
-      {init last:  St}
-      (D:          HSEMechanism S C)
-      (r:          Run C init last):
+      {H E S:     Type}
+     `{Event      E}
+      {C:   ComputingSystem H E}
+      {init last: H}
+      (D:         HSEMechanism S C)
+      (r:         Run C init last):
     compliant_run D r -> state_inv D last.
 Proof.
   induction r.
   + unfold compliant_run.
     intros [Hinv Hb].
     destruct Hst as [Hpre Hpost].
-    apply (behavior_preserves_state_inv D init last ev Hinv Hb Hpre Hpost).
+    apply (preserves_state_inv D init last ev Hinv Hpre Hb Hpost).
   + intros Hcomp.
     inversion Hcomp as [Hinv Hb].
     inversion Hb as [H1 H2].
     apply compliant_run_unwrap in Hcomp.
     apply IHr in Hcomp.
     destruct Hst as [Hpre Hpost].
-    apply (behavior_preserves_state_inv D penultimate last ev Hcomp H2 Hpre Hpost).
+    apply (preserves_state_inv D penultimate last ev Hcomp Hpre H2 Hpost).
 Qed.
