src/x86/Event.v
@@ -1,27 +1,97 @@
+Require Import Program.
+
 Require Import SpecCert.x86.Architecture.
 Require Import SpecCert.x86.Value.
 Require Import SpecCert.Address.
 Require Import SpecCert.Formalism.
+Require Import SpecCert.Utils.
 
 (* A software event is an event produced by the execution of an
  * assembly instruction.
- *)
-Inductive SoftwareEvent :=
-| DisableInterrupt :SoftwareEvent
-| EnableInterrupt  :SoftwareEvent
-| Read             :PhysicalAddress -> Value -> SoftwareEvent
-| Write            :PhysicalAddress -> Value -> SoftwareEvent
-| OpenSmram        :SoftwareEvent
-| CloseSmram       :SoftwareEvent
-| LockSmramc       :SoftwareEvent
-| NextInstruction  :PhysicalAddress -> SoftwareEvent.
-
-(* A hardware event is an event produced by the hardware in response
+ *
+ * A hardware event is an event produced by the hardware in response
  * to *something*. It can interrupt the normal execution flow of an
- * assembly instruction, for instance
- *)
-Inductive HardwareEvent :=
-| Exec             :Value -> HardwareEvent
-| ReceiveInterrupt :Interrupt -> HardwareEvent.
+ * assembly instruction, for instance *)
+Inductive x86Event :=
+| DisableInterrupt: x86Event
+| EnableInterrupt:  x86Event
+| Read:             PhysicalAddress -> Value -> x86Event
+| Write:            PhysicalAddress -> Value -> x86Event
+| OpenSmram:        x86Event
+| CloseSmram:       x86Event
+| LockSmramc:       x86Event
+| NextInstruction:  PhysicalAddress -> x86Event
+| Exec:             Value -> x86Event
+| ReceiveInterrupt: Interrupt -> x86Event.
+Definition x86_software
+           (e: x86Event)
+  : Prop :=
+  match e with
+  | DisableInterrupt  => True
+  | EnableInterrupt   => True
+  | Read _ _          => True
+  | Write _ _         => True
+  | OpenSmram         => True
+  | CloseSmram        => True
+  | LockSmramc        => True
+  | NextInstruction _ => True
+  | _                 => False
+  end.
 
-Definition x86Event := Event SoftwareEvent HardwareEvent.
+Program Definition x86_software_dec
+           (e: x86Event)
+  : { x86_software e } + { ~ x86_software e } :=
+  match e with
+  | DisableInterrupt   => true_dec
+  | EnableInterrupt    => true_dec
+  | Read _ _           => true_dec
+  | Write _ _          => true_dec
+  | OpenSmram          => true_dec
+  | CloseSmram         => true_dec
+  | LockSmramc         => true_dec
+  | NextInstruction _  => true_dec
+  | Exec _             => false_dec
+  | ReceiveInterrupt _ => false_dec
+  end.
+
+Instance X86Event: Event x86Event :=
+  { software := x86_software
+  ; software_dec := x86_software_dec
+  }.
+
+Program Definition DisableInterrupt'
+  : { e: x86Event | x86_software e }
+  := DisableInterrupt.
+
+Program Definition EnableInterrupt'
+  : { e: x86Event | x86_software e }
+  := EnableInterrupt.
+
+Program Definition Read'
+        (pa: PhysicalAddress)
+        (v:  Value)
+  : { e: x86Event | x86_software e }
+  := Read pa v.
+
+Program Definition Write'
+        (pa: PhysicalAddress)
+        (v:  Value)
+  : { e: x86Event | x86_software e }
+  := Write pa v.
+
+Program Definition OpenSmram'
+  : { e: x86Event | x86_software e }
+  := OpenSmram.
+
+Program Definition CloseSmram'
+  : { e: x86Event | x86_software e }
+  := CloseSmram.
+
+Program Definition LockSmram'
+  : { e: x86Event | x86_software e }
+  := LockSmramc.
+
+Program Definition NextInstruction'
+        (pa: PhysicalAddress)
+  : { e: x86Event | x86_software e }
+  := NextInstruction pa.
