src/Smm/Delta/Preserve/Preserve_proofs.v
@@ -1,3 +1,5 @@
+Require Import Program.
+
 Require Import SpecCert.Formalism.
 Require Import SpecCert.Smm.Delta.Invariant.
 Require Import SpecCert.Smm.Delta.Preserve.CloseSmram.
@@ -11,24 +13,37 @@ Require Import SpecCert.Smm.Delta.Preserve.ReceiveInterrupt.
 Require Import SpecCert.Smm.Delta.Preserve.Write.
 Require Import SpecCert.x86.
 
-Theorem software_transitions_preserve_inv:
-  forall ev :SoftwareEvent,
-    software_preserve_inv ev.
+Program Theorem software_transitions_preserve_inv
+        (ev: { e: x86Event | x86_software e })
+  : software_preserve_inv ev.
 Proof.
-  induction ev; unfold software_preserve_inv; intros a a' Hinv Hsmm Htrans.
+  induction ev as [ev Hev]; induction ev;
+    unfold software_preserve_inv;
+    intros a a' Hinv Hsmm Htrans;
+    simpl in *;
+    try destruct Hev. (* deal with hardware events very quickly *)
   + apply (disable_interrupt_inv a a' Hinv Htrans).
   + apply (enable_interrupt_inv a a' Hinv Htrans).
-  + eapply (read_inv _ _ a a' Hinv Htrans).
+  + apply (read_inv _ _ a a' Hinv Htrans).
   + apply (write_inv _ _ a a' Hinv Htrans).
   + apply (open_smram_inv a a' Hinv Htrans).
   + apply (close_smram_inv a a' Hinv Htrans).
   + apply (lock_smramc_inv a a' Hinv Htrans).
-  + eapply (nextinstr_inv _ a a' Hinv Hsmm Htrans).
+  + apply (nextinstr_inv _ a a' Hinv Hsmm Htrans).
 Qed.
 
-Theorem hardware_transitions_preserve_inv: forall ev, preserve_inv (hardware ev).
+Program Theorem hardware_transitions_preserve_inv
+        (ev : { ev: x86Event | ~ x86_software ev })
+  : preserve_inv ev.
 Proof.
-  induction ev.
+  (* TODO We have to find a better way to discard software event *)
+  assert ((~ True) -> False) as H by (intuition).
+  induction ev as [ev Hev];
+    induction ev;
+    try (simpl in Hev;
+         assert (~ True) as H' by (exact Hev);
+         apply H in H';
+         destruct H'); simpl in *.
   + apply exec_inv.
   + apply receive_interrupt_inv.
 Qed.
