src/Smm/Delta/Preserve/ReceiveInterrupt.v
@@ -3,15 +3,15 @@ Require Import SpecCert.Smm.Delta.Invariant.
 Require Import SpecCert.Smm.Software.
 Require Import SpecCert.x86.
 
-Lemma receive_interrupt_inv:
-  forall i :Interrupt,
-    preserve_inv (hardware (ReceiveInterrupt i)).
+Lemma receive_interrupt_inv
+      (i: Interrupt)
+  : preserve_inv (ReceiveInterrupt i).
 Proof.
   unfold preserve_inv.
   unfold inv.
   unfold smramc_inv, smram_code_inv, smrr_inv, cache_clean_inv, ip_inv, smbase_inv.
   unfold context.
-  intros i a a' [Hsmramc [Hsmram [Hsmrr [Hclean [Hip Hsmbase]]]]] Hpre Hpost.
+  intros a a' [Hsmramc [Hsmram [Hsmrr [Hclean [Hip Hsmbase]]]]] Hpre Hpost.
   unfold x86_postcondition, receive_interrupt_post, receive_interrupt, receive_smi in Hpost.
   destruct (will_process_interrupt_dec (proc a) i);
     destruct i;
