src/Smm/Delta/Secure/ReceiveInterrupt.v
@@ -6,9 +6,9 @@ Require Import SpecCert.Smm.Delta.Secure.Secure_def.
 Require Import SpecCert.Smm.Software.
 Require Import SpecCert.x86.
 
-Lemma receive_interrupt_inv_is_secure: forall i:Interrupt,
-  inv_is_secure (hardware (ReceiveInterrupt i)).
+Lemma receive_interrupt_inv_is_secure
+      (i: Interrupt)
+  : inv_is_secure (ReceiveInterrupt i).
 Proof.
-  intro i.
   trivial_inv_is_secure.
 Qed.
