src/Smm/Delta/Secure/Secure_proofs.v
@@ -1,27 +1,29 @@
 Require Import SpecCert.Formalism.
-Require Import SpecCert.Smm.Delta.Secure.Secure_def.
-Require Import SpecCert.Smm.Delta.Secure.EnableInterrupt.
-Require Import SpecCert.Smm.Delta.Secure.DisableInterrupt.
-Require Import SpecCert.Smm.Delta.Secure.ReceiveInterrupt.
-Require Import SpecCert.Smm.Delta.Secure.Read.
-Require Import SpecCert.Smm.Delta.Secure.Write.
-Require Import SpecCert.Smm.Delta.Secure.OpenSmram.
 Require Import SpecCert.Smm.Delta.Secure.CloseSmram.
+Require Import SpecCert.Smm.Delta.Secure.DisableInterrupt.
+Require Import SpecCert.Smm.Delta.Secure.EnableInterrupt.
 Require Import SpecCert.Smm.Delta.Secure.LockSmramc.
 Require Import SpecCert.Smm.Delta.Secure.NextInstruction.
+Require Import SpecCert.Smm.Delta.Secure.OpenSmram.
+Require Import SpecCert.Smm.Delta.Secure.Read.
+Require Import SpecCert.Smm.Delta.Secure.ReceiveInterrupt.
+Require Import SpecCert.Smm.Delta.Secure.Secure_def.
+Require Import SpecCert.Smm.Delta.Secure.Write.
+Require Import SpecCert.x86.
 
-Theorem invariant_permits_security: forall ev, inv_is_secure ev.
+Program Theorem invariant_permits_security
+        (ev: x86Event)
+  : inv_is_secure ev.
 Proof.
-  induction ev as [s|h]; [
-  induction s ;[
-       apply disable_interrupt_inv_is_secure
-     | apply enable_interrupt_inv_is_secure
-     | apply read_inv_is_secure
-     | apply write_inv_is_secure
-     | apply open_smram_inv_is_secure
-     | apply close_smram_inv_is_secure
-     | apply lock_smramc_inv_is_secure
-     | apply nextinstr_inv_is_secure ]
-  | induction h; [ apply exec_inv_is_secure
-                 | apply receive_interrupt_inv_is_secure ]].
+  induction ev;
+    [ apply disable_interrupt_inv_is_secure
+    | apply enable_interrupt_inv_is_secure
+    | apply read_inv_is_secure
+    | apply write_inv_is_secure
+    | apply open_smram_inv_is_secure
+    | apply close_smram_inv_is_secure
+    | apply lock_smramc_inv_is_secure
+    | apply nextinstr_inv_is_secure
+    | apply exec_inv_is_secure
+    | apply receive_interrupt_inv_is_secure ].
 Qed.
